rocq-osiris/theories/program_logic/rules/expr_rules.v
@@ -275,6 +275,60 @@ Section imp_rules_expr.
   (** * ERecord : list fexpr → expr *)
   (** * ERecordUpdate : expr → list fexpr → expr *)
   (** * ERecordAccess : expr → field → expr *)
+
+  (** * EFreeze : expr → expr *)
+
+  Lemma imp_EFreeze2 {ζ} (Φ : block → list loc → iProp Σ) (Φ' : block → iProp Σ) η e :
+    impure E (eval η e) Ψ ζ Φ' -∗
+    (∀ l, Φ' l -∗ ∃ t ls, isBlock l (DfracOwn 1) t ls ∗ Φ l ls) -∗
+    impure E (eval η (EFreeze e)) Ψ ζ (λ l, ∃ ls, Φ l ls ∗ isBlock l (DfracOwn 1) Immut ls).
+  Proof.
+    iIntros "He Hcov".
+    simpl_eval.
+    iApply (imp_bind with "[He]").
+    { iApply (imp_as_block with "He"). }
+    iIntros (l) "HΦl".
+    iDestruct ("Hcov" with "HΦl") as "(%t & %ls & Hl & HΦ)".
+    iApply (imp_bind with "[Hl]").
+    { iApply (imp_set_tag with "Hl"). }
+    iIntros ([]) "Hl".
+    iApply imp_ret; first encode.
+    iFrame.
+  Qed.
+
+  Lemma imp_EFreeze {ζ} l t ls η e :
+    isBlock l (DfracOwn 1) t ls -∗
+    impure E (eval η e) Ψ ζ (λ l', ⌜l' = l⌝) -∗
+    impure E (eval η (EFreeze e)) Ψ ζ (λ l', ⌜l' = l⌝ ∗ isBlock l (DfracOwn 1) Immut ls).
+  Proof.
+    iIntros "Hl He".
+    iApply (imp_wand with "[-]").
+    { iApply (imp_EFreeze2 (λ l' ls', ⌜l' = l⌝ ∗ ⌜ls' = ls⌝)%I with "He").
+      iIntros (?) "->". by iFrame. }
+    iIntros (?) "(% & (-> & ->) & $)".
+    auto.
+  Qed.
+
+  (** * EUnfreeze : expr → expr *)
+
+  Lemma imp_EUnfreeze {ζ} (Φ' : block → iProp Σ) (Φ : block → list loc → iProp Σ) η e :
+    impure E (eval η e) Ψ ζ Φ' -∗
+    (∀ l, Φ' l -∗ ∃ t ls, isBlock l (DfracOwn 1) t ls ∗ Φ l ls) -∗
+    impure E (eval η (EUnfreeze e)) Ψ ζ (λ l, ∃ ls, Φ l ls ∗ isBlock l (DfracOwn 1) Mut ls).
+  Proof.
+    iIntros "He Hcov".
+    simpl_eval.
+    iApply (imp_bind with "[He]").
+    { iApply (imp_as_block with "He"). }
+    iIntros (l) "HΦl".
+    iDestruct ("Hcov" with "HΦl") as "(%t & %ls & Hl & HΦ)".
+    iApply (imp_bind with "[Hl]").
+    { iApply (imp_set_tag with "Hl"). }
+    iIntros ([]) "Hl".
+    iApply imp_ret; first encode.
+    iFrame.
+  Qed.
+
   (** * EBoolConj : expr → expr → expr *)
   (** * EBoolDisj : expr → expr → expr *)
   (** * EBoolNeg : expr → expr *)
